src/go_lang/StructTests.v
@@ -1,0 +1,30 @@
+From Perennial.go_lang Require Import notation struct.
+
+Section go_lang.
+  Context `{ffi_sem: ext_semantics}.
+
+  Definition threeS := struct ["foo"; "bar"; "baz"].
+
+  Definition Foo: val := structF! threeS "foo".
+  Definition Bar: val := structF! threeS "bar".
+  Fail Definition Quux: val := structF! threeS "quux".
+
+  Ltac goal_is_exactly_equal :=
+    lazymatch goal with
+    | [ |- ?a = ?a ] => reflexivity
+    | [ |- ?a = ?b ] => idtac a "is not" b; fail "not an exact match"
+    | _ => fail "unexpected goal"
+    end.
+
+  Theorem Foo_is : Foo = (λ: "v", Fst (Fst (Var' "v")))%V.
+  Proof.
+    unfold Foo.
+    goal_is_exactly_equal.
+  Qed.
+
+  Theorem Bar_is : Bar = (λ: "v", Fst (Snd (Var' "v")))%V.
+  Proof.
+    unfold Bar.
+    goal_is_exactly_equal.
+  Qed.
+End go_lang.
