src/go_lang/examples/logging.v
@@ -1,101 +1,23 @@
 From iris.proofmode Require Import tactics.
 From iris.program_logic Require Export weakestpre.
-From Perennial.go_lang Require Export lang.
+From Perennial.go_lang Require Export lang struct slice.
 From Perennial.go_lang Require Export ffi.disk.
 From Perennial.go_lang Require Import proofmode notation.
 
 Existing Instances disk_op disk_model disk_semantics disk_interp.
 
-Coercion Var' (s: string) : expr := Var s.
+Local Coercion Var' (s: string) : expr := Var s.
 
-(** Lightweight struct library: access field offsets within pairs by name rather
-than using prod projections. *)
+(** * Append-only, seqeuntial, crash-safe log.
 
-Record descriptor :=
-  struct { fields: list string; }.
-
-(* Check eq_refl : (#0, #1, #2)%E = ((#0, #1), #2)%E. *)
-
-Fixpoint get_field_e (f0: string) (rev_fields: list string): expr :=
-  match rev_fields with
-  | nil => #()
-  | [f] => if String.eqb f f0 then "v" else #()
-  | f::fs => if String.eqb f f0 then Snd "v" else Fst (get_field_e f0 fs)
-  end.
-
-Definition get_field (d:descriptor) f : val :=
-  λ: "v", get_field_e f (rev d.(fields)).
-
-Ltac make_structF desc fname :=
-  let f := eval compute [desc get_field rev app get_field_e fields String.eqb Ascii.eqb eqb]
-  in (get_field desc fname) in
-      lazymatch f with
-      | context[LitUnit] => fail "struct" desc "does not have field" fname
-      | _ => exact f
-      end.
-
-Notation "'structF!' desc fname" := (ltac:(make_structF desc fname))
-                                    (at level 0, desc, fname at next level, only parsing) : val_scope.
-
-(** Slice library, for manipulating (pointer, len) structs. *)
-
-Definition sliceS := struct ["p"; "len"].
-
-(*
-Eval compute in get_field sliceS "p".
-Eval compute in get_field sliceS "len".
-*)
-
-Definition NewByteSlice: val :=
-  λ: "sz",
-  let: "p" := AllocN "sz" #(LitByte 0) in
-  ("p", "sz").
-
-Definition SlicePtr: val := structF! sliceS "p".
-Definition SliceLen: val := structF! sliceS "len".
-
-Definition For (v:string) (bound:expr) (body:expr) : expr :=
-  (rec: "__loop" v :=
-     if: v < bound then body v;; "__loop" (v + #1) else #()) #0.
-
-Notation "'for:' v < b := e" := (For v%string b%E e%E)
-  (at level 200, v at level 1, b at level 1, e at level 200,
-   format "'[' 'for:'  v  <  b  :=  '/  ' e ']'") : expr_scope.
-
-Definition MemCpy: val :=
-  λ: "dst" "src" "n",
-    for: "i" < "n" :=
-    ("dst" +ₗ "i") <- !("src" +ₗ "i").
-
-(* explicitly recursive version of MemCpy *)
-Definition MemCpy_rec: val :=
-  rec: "memcpy" "dst" "src" "n" :=
-    if: "n" = #0
-    then #()
-    else "dst" <- !"src";;
-         "memcpy" ("dst" +ₗ #1) ("src" +ₗ #1) ("n" - #1).
-
-Definition SliceSkip: val :=
-  λ: "s" "n", (SlicePtr "s" +ₗ "n", SliceLen "s" - "n").
-
-Definition SliceTake: val :=
-  λ: "s" "n", if: SliceLen "s" < "n"
-              then #() (* TODO: this should be Panic *)
-              else (SlicePtr "s", "n").
-
-Definition SliceGet: val :=
-  λ: "s" "i",
-  !(SlicePtr "s" +ₗ "i").
-
-Definition SliceAppend: val :=
-  λ: "s1" "s2",
-  let: "p" := AllocN (SliceLen "s1" + SliceLen "s2") #() in
-  MemCpy "p" (SlicePtr "s1");;
-  MemCpy ("p" +ₗ SliceLen "s2") (SlicePtr "s2");;
-  (* TODO: unsound, need to de-allocate s1.p *)
-  ("p", SliceLen "s1" + SliceLen "s2").
+    The main interesting feature is that the log supports multi-block atomic
+    appends, which are implemented by atomically updating an on-disk header with
+    the number of valid blocks in the log.
+ *)
 
 Definition logS := struct ["log_sz"; "disk_sz"].
+Definition LogSize: val := structF! logS "log_sz".
+Definition DiskSize: val := structF! logS "disk_sz".
 
 Definition write_hdr: val :=
   λ: "log",
@@ -111,9 +33,6 @@ Definition init: val :=
     let: "log" := (#0, "disk_sz") in
     write_hdr "log";;
     SOME "log".
-
-Definition LogSize: val := structF! logS "log_sz".
-Definition DiskSize: val := structF! logS "disk_sz".
 
 Definition get: val :=
   λ: "log" "i",
