src/go_lang/notation.v
@@ -39,6 +39,7 @@ Notation CAS l e1 e2 := (Snd (CmpXchg l e1 e2)) (only parsing).
    it. Hence, we need to explicitly use LamV instead of e.g., Seq. *)
 Notation Skip := (App (Val $ LamV BAnon (Val $ LitV LitUnit)) (Val $ LitV LitUnit)).
 
+
 (* No scope for the values, does not conflict and scope is often not inferred
 properly. *)
 Notation "# l" := (LitV l%Z%V%stdpp) (at level 8, format "# l").
@@ -169,3 +170,10 @@ Notation "'match:' e0 'with' 'SOME' x => e2 | 'NONE' => e1 'end'" :=
 
 Notation ResolveProph e1 e2 := (Resolve Skip e1 e2) (only parsing).
 Notation "'resolve_proph:' p 'to:' v" := (ResolveProph p v) (at level 100) : expr_scope.
+
+Definition For {ext:ext_op} (v:string) (bound:expr) (body:expr) : expr :=
+  (rec: "__loop" v :=
+     if: Var v < bound then body (Var v);; (Var "__loop") (Var v + #1) else #()) #0.
+Notation "'for:' v < b := e" := (For v%string b%E e%E)
+  (at level 200, v at level 1, b at level 1, e at level 200,
+   format "'[' 'for:'  v  <  b  :=  '/  ' e ']'") : expr_scope.
