src/go_lang/slice.v
@@ -1,0 +1,64 @@
+From Perennial.go_lang Require Export lang notation.
+From Perennial.go_lang Require Import notation struct.
+
+(** * Slice library
+
+    Intended to model Go slices. We don't track slice capacity because our model
+    soundly approximates slices as never having extra capacity.
+ *)
+
+Definition sliceS := struct ["p"; "len"].
+
+(*
+Eval compute in get_field sliceS "p".
+Eval compute in get_field sliceS "len".
+*)
+
+Section go_lang.
+  Context `{ffi_sem: ext_semantics}.
+
+  Definition Var' s : @expr ext := Var s.
+  Local Coercion Var' : string >-> expr.
+
+Definition NewByteSlice: val :=
+  λ: "sz",
+  let: "p" := AllocN "sz" #(LitByte 0) in
+  ("p", "sz").
+
+Definition SlicePtr: val := structF! sliceS "p".
+Definition SliceLen: val := structF! sliceS "len".
+
+Definition MemCpy: val :=
+  λ: "dst" "src" "n",
+    for: "i" < "n" :=
+    ("dst" +ₗ "i") <- !("src" +ₗ "i").
+
+(* explicitly recursive version of MemCpy *)
+Definition MemCpy_rec: val :=
+  rec: "memcpy" "dst" "src" "n" :=
+    if: "n" = #0
+    then #()
+    else "dst" <- !"src";;
+         "memcpy" ("dst" +ₗ #1) ("src" +ₗ #1) ("n" - #1).
+
+Definition SliceSkip: val :=
+  λ: "s" "n", (SlicePtr "s" +ₗ "n", SliceLen "s" - "n").
+
+Definition SliceTake: val :=
+  λ: "s" "n", if: SliceLen "s" < "n"
+              then #() (* TODO: this should be Panic *)
+              else (SlicePtr "s", "n").
+
+Definition SliceGet: val :=
+  λ: "s" "i",
+  !(SlicePtr "s" +ₗ "i").
+
+Definition SliceAppend: val :=
+  λ: "s1" "s2",
+  let: "p" := AllocN (SliceLen "s1" + SliceLen "s2") #() in
+  MemCpy "p" (SlicePtr "s1");;
+  MemCpy ("p" +ₗ SliceLen "s2") (SlicePtr "s2");;
+  (* TODO: unsound, need to de-allocate s1.p *)
+  ("p", SliceLen "s1" + SliceLen "s2").
+
+End go_lang.
