src/go_lang/struct.v
@@ -1,0 +1,40 @@
+From Perennial.go_lang Require Export lang.
+From Perennial.go_lang Require Import notation.
+
+(** * Lightweight struct library
+
+    Access field offsets within pairs by name rather than using Fst and Snd. *)
+
+Record descriptor :=
+  struct { fields: list string; }.
+
+(* Check eq_refl : (#0, #1, #2)%E = ((#0, #1), #2)%E. *)
+
+Section go_lang.
+  Context `{ffi_sem: ext_semantics}.
+
+  Definition Var' s : @expr ext := Var s.
+  Local Coercion Var' : string >-> expr.
+
+Fixpoint get_field_e (f0: string) (rev_fields: list string): expr :=
+  match rev_fields with
+  | nil => LitV LitUnit
+  | [f] => if String.eqb f f0 then "v" else #()
+  | f::fs => if String.eqb f f0 then Snd "v" else Fst (get_field_e f0 fs)
+  end.
+
+Definition get_field (d:descriptor) f : val :=
+  λ: "v", get_field_e f (rev d.(fields)).
+
+End go_lang.
+
+Ltac make_structF desc fname :=
+  let f := eval compute [desc get_field rev app get_field_e fields String.eqb Ascii.eqb eqb]
+  in (get_field desc fname) in
+      lazymatch f with
+      | context[LitUnit] => fail "struct" desc "does not have field" fname
+      | _ => exact f
+      end.
+
+Notation "'structF!' desc fname" := (ltac:(make_structF desc fname))
+                                    (at level 0, desc, fname at next level, only parsing) : val_scope.
